DesmosFormalization/Expr.lean
@@ -1,0 +1,46 @@
+import DesmosFormalization.Types
+import DesmosFormalization.Wackscope
+import DesmosFormalization.Infer
+
+inductive Value
+  | bool   : Bool -> Value
+  | number : Float -> Value
+  | point  : Float -> Float -> Value
+  deriving Repr
+
+inductive HasType : Value -> Ty -> Prop
+ | htBool    : HasType (.bool b)    .bool
+ | htNum     : HasType (.number n)  .number
+ | htPoint : HasType (.point x y) .point
+
+def VarExprEnv := Name -> Option Expr
+def FnExprEnv  := Name -> Option (Name -> Name -> Expr)
+
+def evalOp : BinOp -> Value -> Value -> Option Value
+  | .add, .number x, .number y =>
+      some (.number (x + y))
+  | .add, .point x₁ y₁, .point x₂ y₂ =>
+      some (.point (x₁ + x₂) (y₁ + y₂))
+  | .dot, .number x, .number y =>
+      some (.number (x * y))
+  | .dot, .point x₁ y₁, .point x₂ y₂ =>
+      some (.number (x₁ * x₂ + y₁ * y₂))
+  | .dot, .number s, .point x y =>
+      some (.point (s * x) (s * y))
+  | .dot, .point x y, .number s =>
+      some (.point (s * x) (s * y))
+  | .point, .number x, .number y =>
+      some (.point x y)
+  | .leq, .number x, .number y =>
+      some (.bool (x <= y))
+  | _, _, _ =>
+      none
+
+def evalVar (x : Name) (Γvar : VarExprEnv) (Γfn : FnExprEnv) : Option Value := do
+  let expr <- Γvar x
+  evalExpr expr
+
+
+  some (.number 5)
+
+def evalExpr 
