DesmosFormalization/Soundness.lean
@@ -1,0 +1,198 @@
+import DesmosFormalization.Types
+import DesmosFormalization.Wackscope
+import DesmosFormalization.Infer
+
+abbrev Assignment := Name -> Ty
+
+def Agrees (σ : Assignment) (s : Scheme) (case : Ty × (s.deps -> Ty))
+  : Prop :=
+  ∀ d : s.deps, σ d = case.2 d
+
+
+
+inductive HasType :
+  VarEnv -> FnEnv -> Assignment -> Expr -> Ty -> Prop
+
+  | var_defined
+    (Γv Γf σ x s case τ)
+    (hlookup : Γv x = some s)
+    (hmem    : case ∈ s.scheme)
+    (hagree  : Agrees σ s case)
+    (hτ      : τ = case.1) :
+    HasType Γv Γf σ (.var x) τ
+
+  | var_free
+    (Γv Γf σ x)
+    (hLookup : Γv x = none) :
+    HasType Γv Γf σ (.var x) (σ x)
+
+  | lit : HasType Γv Γf σ (.lit x) .number
+
+  | add_number
+    (h₁ : HasType Γv Γf σ e₁ .number)
+    (h₂ : HasType Γv Γf σ e₂ .number) :
+    HasType Γv Γf σ (.binop e₁ e₂ .add) .number
+
+  | add_point
+    (h₁ : HasType Γv Γf σ e₁ .point)
+    (h₂ : HasType Γv Γf σ e₂ .point) :
+    HasType Γv Γf σ (.binop e₁ e₂ .add) .point
+
+  | call
+    (hlookup : Γf f = some s)
+    (hmem    : case ∈ s.scheme)
+    (hagree  : ∀ d : s.deps, σ d = case.2 d)
+    :
+    HasType Γv Γf σ (.call f e₁ e₂) τret
+
+def SchemeDenotes Γv Γf e (s : Scheme) :=
+  ∀ σ τ,
+    HasType Γv Γf σ e τ
+    ↔
+    (τ, fun x : s.deps => σ x) ∈ s.scheme
+
+lemma freeVarScheme_complete :
+  ∀ σ x,
+    ∃ case ∈ (Scheme.freeVar x).scheme,
+    case.1 = σ x ∧ Agrees σ _ case := by sorry
+
+theorem inferExpr_sound :
+  inferExpr Γv Γf e = s -> SchemeDenotes Γv Γf e s := by
+  induction e generalizing s
+  case var x =>
+    intro hEq
+    simp [inferExpr] at hEq
+    unfold SchemeDenotes
+    intro σ τ
+    apply Iff.intro
+    · intro hType
+      cases hType with
+      | var_defined Γv Γf σ x s case τ hlookup hmem hagree hτ =>
+        simp [hlookup] at hEq
+        unfold Agrees at hagree
+        aesop
+      | var_free Γv Γf σ x hlookup =>
+        rw [hlookup] at hEq
+        simp at hEq
+        have hsingleton : s.deps = { x } := by
+          rw [<-hEq]
+          unfold Scheme.freeVar
+          simp
+        have hfun : (fun x₁ : s.deps => σ x₁) = (fun x₁ => σ x) := by
+          grind
+        rw [hfun]
+        rw [<-hEq]
+        unfold Scheme.freeVar
+        unfold allTys
+        cases σ x
+        grind
+        grind
+        grind
+
+    · cases hlookup : Γv x
+      rw [hlookup] at hEq
+      simp at hEq
+      rw [<-hEq]
+      intro hmem
+      rcases List.mem_map.mp hmem with ⟨τ', hτ', hpair⟩
+      injection hpair with hτeq hfun
+      have hσx : τ = σ x := by
+        rw [<-hτeq]
+        have := congrArg (fun f => f ⟨x, by grind⟩) hfun
+        simp at this
+        exact this
+      rw [hσx]
+      apply HasType.var_free
+      exact hlookup
+
+      rw [hlookup] at hEq
+      simp at hEq
+      intro hmem
+      -- have case :=
+      apply HasType.var_defined Γv Γf σ x s (τ, (σ ·)) τ
+      rw [hEq] at hlookup
+      exact hlookup
+      exact Multiset.mem_coe.mp hmem
+      exact (congrFun ∘ fun a => a) rfl
+      exact ((fun a => a) ∘ fun a => a) rfl
+
+  case lit x =>
+    intro hEq
+    simp [inferExpr] at hEq
+    unfold SchemeDenotes
+    intro σ τ
+    apply Iff.intro
+    intro hType
+    cases hType
+    rw [<-hEq]
+    simp
+    aesop
+
+    intro hmem
+    rw [<-hEq] at hmem
+    simp at hmem
+    rw [hmem.1]
+    apply HasType.lit
+
+  case binop e₁ e₂ op ih₁ ih₂ =>
+    intro hEq
+    simp [inferExpr] at hEq
+    let s₁ := inferExpr Γv Γf e₁
+    let s₂ := inferExpr Γv Γf e₂
+    have h₁ : SchemeDenotes Γv Γf e₁ s₁ := by
+      exact (ih₁ ∘ congrArg (inferExpr Γv Γf)) rfl
+    have h₂ : SchemeDenotes Γv Γf e₂ s₂ := by
+      exact (ih₂ ∘ congrArg (inferExpr Γv Γf)) rfl
+    intro σ τ
+
+    apply Iff.intro
+    
+
+
+
+
+    -- apply HasType.lit Γv Γf σ (.lit x) .number
+
+
+
+
+
+
+
+      -- have case := (τ, fun x : ↥s.deps => σ x)
+
+
+
+
+
+
+
+
+
+
+
+
+
+
+
+      -- cases hσ : σ x
+      -- simp [Scheme.freeVar, hσ]
+
+      -- have hfun : (fun x₁ => σ ↑x₁) = (fun _ => Ty.bool) := by
+      --   funext x₁
+
+
+
+
+
+    -- cases hlookup
+    -- simp at hEq
+
+    -- cases hType
+
+
+
+
+
+
+-- theorem soundness
